better factoring-out of mul_converted stuff, define saturated arith operations

src/Experiments/SimplyTypedArithmetic.v
@@ -1017,6 +1017,7 @@ Module Rows.
     Local Notation cols := (list (list Z)) (only parsing).
 
     Hint Rewrite Positional.eval_nil Positional.eval0 @Positional.eval_snoc
+         Positional.eval_to_associational
          Columns.eval_nil Columns.eval_snoc using (auto; solve [distr_length]) : push_eval.
     Hint Resolve in_eq in_cons.
     Hint Resolve Z.gt_lt.
@@ -1206,6 +1207,65 @@ Module Rows.
         match goal with H: _ |- _ => apply length_from_columns in H end.
         rewrite Columns.length_from_associational in *; auto.
       Qed.
+
+      (* TODO : move *)
+      Lemma max_0_iff a b : Nat.max a b = 0%nat <-> (a = 0%nat /\ b = 0%nat).
+      Proof.
+        destruct a, b; try tauto.
+        rewrite <-Nat.succ_max_distr.
+        split; [ | destruct 1]; congruence.
+      Qed.
+      Lemma max_column_size_zero_iff x :
+        max_column_size x = 0%nat <-> (forall c, In c x -> c = nil).
+      Proof.
+        cbv [max_column_size]; induction x; intros; [ cbn; tauto | ].
+        autorewrite with push_fold_right push_map.
+        rewrite max_0_iff, IHx.
+        split; intros; [ | rewrite length_zero_iff_nil; solve [auto] ].
+        match goal with H : _ /\ _ |- _ => destruct H end.
+        In_cases; subst; auto using length0_nil.
+      Qed.
+
+      Lemma Columns_from_associational_step n t p :
+        Columns.from_associational weight n (t :: p) =
+        Columns.cons_to_nth (fst (Positional.place weight t (Nat.pred n)))
+                            (snd (Positional.place weight t (Nat.pred n)))
+                            (Columns.from_associational weight n p).
+      Admitted.
+
+      Lemma max_column_size_Columns_from_associational n p :
+        n <> 0%nat -> p <> nil ->
+        max_column_size (Columns.from_associational weight n p) <> 0%nat.
+      Proof.
+        intros.
+        rewrite max_column_size_zero_iff.
+        intro. destruct p; [congruence | ].
+        rewrite Columns_from_associational_step in *.
+        cbv [Columns.cons_to_nth] in *.
+        match goal with H : forall c, In c (update_nth ?n ?f ?ls) -> _ |- _ =>
+                        assert (n < length (update_nth n f ls))%nat;
+                          [ | specialize (H (nth n (update_nth n f ls) nil) ltac:(auto using nth_In)) ]
+        end.
+        { distr_length.
+          rewrite Columns.length_from_associational.
+          remember (Nat.pred n) as m. replace n with (S m) by omega.
+          apply Positional.place_in_range. }
+        rewrite <-nth_default_eq in *.
+        autorewrite with push_nth_default in *.
+        rewrite eq_nat_dec_refl in *.
+        congruence. 
+      Qed.
+
+      Lemma from_associational_nonnil n p :
+        n <> 0%nat -> p <> nil ->
+        from_associational n p <> nil.
+      Proof.
+        intros; cbv [from_associational from_columns from_columns'].
+        pose proof (max_column_size_Columns_from_associational n p ltac:(auto) ltac:(auto)).
+        case_eq (max_column_size (Columns.from_associational weight n p)); [omega|].
+        intros; cbn.
+        rewrite <-length_zero_iff_nil. distr_length.
+      Qed.
     End FromAssociational.
 
     Section Flatten.
@@ -1360,11 +1420,11 @@ Module Rows.
                       let out_carry := sum_rows next_row (fst state) in
                       (fst out_carry, snd state + snd out_carry)) start_state (rev inp).
 
-      (* For correctness if there is only one row, we add a row of
-         zeroes with the same length so that the add loop still happens. *)
-      Definition flatten (inp : rows) : list Z * Z :=
-        let first_row := hd nil inp in
-        flatten' (first_row, 0) (hd (Positional.zeros (length first_row)) (tl inp) :: tl (tl inp)).
+      (* In order for the output to have the right length and bounds,
+         we insert rows of zeroes if there are fewer than two rows. *)
+      Definition flatten n (inp : rows) : list Z * Z :=
+        let default := Positional.zeros n in
+        flatten' (hd default inp, 0) (hd default (tl inp) :: tl (tl inp)).
 
       Lemma flatten'_cons state r inp :
         flatten' state (r :: inp) = flatten' (fst (sum_rows r (fst state)), snd state + snd (sum_rows r (fst state))) inp.
@@ -1408,20 +1468,24 @@ Module Rows.
 
       Lemma flatten_div_mod inp n :
         (forall row, In row inp -> length row = n) ->
-        is_div_mod (Positional.eval weight n) (flatten inp) (eval n inp) (weight n).
+        is_div_mod (Positional.eval weight n) (flatten n inp) (eval n inp) (weight n).
       Proof.
         intros; cbv [flatten].
-        destruct inp; [|destruct inp]; cbn [hd tl]; try solve [cbv [is_div_mod]; push].
-        eapply is_div_mod_result_equal; try apply flatten'_div_mod_length; push.
+        destruct inp; [|destruct inp]; cbn [hd tl].
+        { cbv [is_div_mod]; push.
+          erewrite sum_rows_div by (distr_length; reflexivity).
+          push. }
+        { cbv [is_div_mod]; push. }
+        { eapply is_div_mod_result_equal; try apply flatten'_div_mod_length; push. }
       Qed.
 
       Lemma flatten_mod inp n :
         (forall row, In row inp -> length row = n) ->
-        Positional.eval weight n (fst (flatten inp)) = (eval n inp) mod (weight n).
+        Positional.eval weight n (fst (flatten n inp)) = (eval n inp) mod (weight n).
       Proof. apply flatten_div_mod. Qed.
       Lemma flatten_div inp n :
         (forall row, In row inp -> length row = n) ->
-        snd (flatten inp) = (eval n inp) / (weight n).
+        snd (flatten n inp) = (eval n inp) / (weight n).
       Proof. apply flatten_div_mod. Qed.
 
       Lemma length_flatten' n start_state inp :
@@ -1433,18 +1497,18 @@ Module Rows.
 
       Lemma length_flatten n inp :
         (forall row, In row inp -> length row = n) ->
-        inp <> nil ->
-        length (fst (flatten inp)) = n.
+        length (fst (flatten n inp)) = n.
       Proof.
-        intros. apply flatten'_div_mod_length; push;
-          destruct inp as [|? [|? ?] ]; try congruence; cbn [hd tl] in *; push.
-        subst row; distr_length; auto.
+        intros.
+        apply length_flatten'; push;
+          destruct inp as [|? [|? ?] ]; try congruence; cbn [hd tl] in *; push;
+            subst row; distr_length.
       Qed. Hint Rewrite length_flatten : distr_length.
 
       Lemma flatten'_partitions n inp : forall start_state,
+        inp <> nil ->
         length (fst start_state) = n ->
         (forall row, In row inp -> length row = n) ->
-        inp <> nil ->
         forall i, (i < n)%nat ->
                   nth_default 0 (fst (flatten' start_state inp)) i
                   = ((Positional.eval weight n (fst start_state) + eval n inp) mod weight (S i)) / (weight i).
@@ -1460,16 +1524,74 @@ Module Rows.
       Lemma flatten_partitions inp n :
         (forall row, In row inp -> length row = n) ->
         forall i, (i < n)%nat ->
-                  nth_default 0 (fst (flatten inp)) i = (eval n inp mod weight (S i)) / (weight i).
+                  nth_default 0 (fst (flatten n inp)) i = (eval n inp mod weight (S i)) / (weight i).
       Proof.
         intros; cbv [flatten].
         intros; destruct inp as [| ? [| ? ?] ]; try congruence; cbn [hd tl] in *;  try solve [push].
-        { cbn. autorewrite with push_nth_default. reflexivity. }
+        { cbn. autorewrite with push_nth_default.
+          rewrite sum_rows_partitions with (n:=n) by distr_length.
+          autorewrite with push_eval zsimplify_fast.
+          auto with zarith. }
         { push. rewrite sum_rows_partitions with (n:=n) by distr_length; push. }
         { rewrite flatten'_partitions with (n:=n); push. }
       Qed.
+
+      Definition partition n x :=
+        map (fun i => (x mod weight (S i)) / weight i) (seq 0 n).
+
+      Lemma nth_default_partitions x : forall p n,
+        (forall i, (i < n)%nat -> nth_default 0 p i = (x mod weight (S i)) / weight i) ->
+        length p = n ->
+        p = partition n x.
+      Proof.
+        cbv [partition]; induction p using rev_ind; intros; distr_length; subst n; [reflexivity|].
+        rewrite Nat.add_1_r, seq_snoc.
+        autorewrite with natsimplify push_map.
+        rewrite <-IHp; auto; intros;
+          match goal with H : context [nth_default _ (p ++ [ _ ])] |- _ =>
+                          rewrite <-H by omega end.
+        { autorewrite with push_nth_default natsimplify. reflexivity. }
+        { autorewrite with push_nth_default natsimplify. 
+          break_match; omega. } 
+      Qed.
+
+      Lemma flatten_partitions' inp n :
+        (forall row, In row inp -> length row = n) ->
+        fst (flatten n inp) = partition n (eval n inp).
+      Proof. auto using nth_default_partitions, flatten_partitions, length_flatten. Qed.
     End Flatten.
 
+    Section Ops.
+      Definition add n p q :=
+        let p_a := Positional.to_associational weight n p in
+        let q_a := Positional.to_associational weight n q in
+        flatten n (from_associational n (p_a ++ q_a)).
+
+      Definition sub n p q :=
+        let p_a := Positional.to_associational weight n p in
+        let q_a := Positional.to_associational weight n q in
+        flatten n (from_associational n (p_a ++ Associational.negate_snd q_a)).
+
+      Lemma add_partitions n p q :
+        n <> 0%nat -> length p = n -> length q = n ->
+        fst (add n p q) = partition n (Positional.eval weight n p + Positional.eval weight n q).
+      Proof.
+        intros; cbv [add].
+        rewrite flatten_partitions' by eauto using length_from_associational.
+        rewrite eval_from_associational by auto.
+        autorewrite with push_eval; reflexivity.
+      Qed.
+
+      Lemma sub_partitions n p q :
+        n <> 0%nat -> length p = n -> length q = n ->
+        fst (sub n p q) = partition n (Positional.eval weight n p - Positional.eval weight n q).
+      Proof.
+        intros; cbv [sub].
+        rewrite flatten_partitions' by eauto using length_from_associational.
+        rewrite eval_from_associational by auto.
+        autorewrite with push_eval; reflexivity.
+      Qed.
+    End Ops.
   End Rows.
 End Rows.
 
@@ -1486,6 +1608,16 @@ Module MulConverted.
               (w_multiples : forall i, w (S i) mod w i = 0)
               (w_divides : forall i : nat, w (S i) / w i > 0).
 
+      (* TODO : move this stuff to BaseConversion *)
+        Definition to_associational n m p : list (Z * Z) :=
+          let p' := BaseConversion.convert_bases w w' n m p in
+          Positional.to_associational w' m p'.
+
+        Definition from_associational idxs n (p : list (Z * Z)) : list Z :=
+          (* important not to use Positional.carry here; we don't want to accumulate yet *)
+          let p' := fold_right (fun i acc => Associational.carry (w' i) (w' (S i) / w' i) acc) p (rev idxs) in
+          fst (Rows.flatten w n (Rows.from_associational w n p')).
+
       (* takes in inputs in base w, converts to w', multiplies in that
          format, converts to w again, then flattens. *)
       Definition mul_converted
@@ -1494,14 +1626,10 @@ Module MulConverted.
               (n3 : nat) (* final length *)
               (idxs : list nat) (* carries to do -- this helps preemptively line up weights *)
               (p1 p2 : list Z) :=
-      let p1' := BaseConversion.convert_bases w w' n1 m1 p1 in
-      let p2' := BaseConversion.convert_bases w w' n2 m2 p2 in
-      let p1_a := Positional.to_associational w' m1 p1' in
-      let p2_a := Positional.to_associational w' m2 p2' in
-      let p3_a := Associational.mul p1_a p2_a in
-      (* important not to use Positional.carry here; we don't want to accumulate yet *)
-      let p3'_a := fold_right (fun i acc => Associational.carry (w' i) (w' (S i) / w' i) acc) p3_a (rev idxs) in
-      fst (Rows.flatten w (Rows.from_associational w n3 p3'_a)).
+        let p1_a := to_associational n1 m1 p1 in
+        let p2_a := to_associational n2 m2 p2 in
+        let p3_a := Associational.mul p1_a p2_a in
+        from_associational idxs n3 p3_a.
 
       Hint Rewrite
            @Rows.eval_from_associational
@@ -1510,55 +1638,95 @@ Module MulConverted.
            @Positional.eval_to_associational
            @BaseConversion.eval_convert_bases using solve [auto using Z.positive_is_nonzero] : push_eval.
 
+      Ltac push_eval := intros; autorewrite with push_eval; auto with zarith.
+
       Lemma eval_carries p idxs :
         Associational.eval (fold_right (fun i acc => Associational.carry (w' i) (w' (S i) / w' i) acc) p idxs) =
         Associational.eval p.
-      Proof. apply fold_right_invariant; intros; autorewrite with push_eval; congruence. Qed.
+      Proof. apply fold_right_invariant; push_eval. Qed.
       Hint Rewrite eval_carries: push_eval.
+
+      Lemma eval_to_associational n m p :
+        m <> 0%nat -> length p = n ->
+        Associational.eval (to_associational n m p) = Positional.eval w n p.
+      Proof. cbv [to_associational]; push_eval. Qed.
+      Hint Rewrite eval_to_associational using solve [push_eval; distr_length] : push_eval.
+
+      Lemma eval_from_associational idxs n p :
+        n <> 0%nat -> 0 <= Associational.eval p < w n ->
+        Positional.eval w n (from_associational idxs n p) = Associational.eval p.
+      Proof.
+        cbv [from_associational]; intros.
+        rewrite Rows.flatten_mod by eauto using Rows.length_from_associational.
+        push_eval.
+      Qed.
+      Hint Rewrite eval_from_associational using solve [push_eval; distr_length] : push_eval.
 
       Lemma eval_mul_converted n1 n2 m1 m2 n3 idxs p1 p2 (_:n3<>0%nat) (_:m1<>0%nat) (_:m2<>0%nat):
         length p1 = n1 -> length p2 = n2 ->
         0 <= (Positional.eval w n1 p1 * Positional.eval w n2 p2) < w n3 ->
         Positional.eval w n3 (mul_converted n1 n2 m1 m2 n3 idxs p1 p2) = (Positional.eval w n1 p1) * (Positional.eval w n2 p2).
-      Proof.
-        cbv [mul_converted]; intros.
-        rewrite Rows.flatten_mod by eauto using Rows.length_from_associational.
-        autorewrite with push_eval. auto using Z.mod_small.
-      Qed.
+      Proof.  cbv [mul_converted]; push_eval. Qed.
       Hint Rewrite eval_mul_converted : push_eval.
 
-      Lemma mul_converted_mod n1 n2 m1 m2 n3 idxs p1 p2  (_:n3<>0%nat) (_:m1<>0%nat) (_:m2<>0%nat):
+      Lemma from_associational_partitions n idxs p  (_:n<>0%nat):
+        forall i, (i < n)%nat ->
+        nth_default 0 (from_associational idxs n p) i = (Associational.eval p) mod (w (S i)) / w i.
+      Proof.
+        intros; cbv [from_associational].
+        rewrite Rows.flatten_partitions with (n:=n) by (eauto using Rows.length_from_associational; omega).
+        push_eval.
+      Qed.
+
+      Lemma mul_converted_partitions n1 n2 m1 m2 n3 idxs p1 p2  (_:n3<>0%nat) (_:m1<>0%nat) (_:m2<>0%nat):
         length p1 = n1 -> length p2 = n2 ->
-        0 <= (Positional.eval w n1 p1 * Positional.eval w n2 p2) < w n3 ->
-        nth_default 0 (mul_converted n1 n2 m1 m2 n3 idxs p1 p2) 0 = (Positional.eval w n1 p1 * Positional.eval w n2 p2) mod (w 1).
+        forall i, (i < n3)%nat ->
+        nth_default 0 (mul_converted n1 n2 m1 m2 n3 idxs p1 p2) i = (Positional.eval w n1 p1 * Positional.eval w n2 p2) mod (w (S i)) / w i.
       Proof.
         intros; cbv [mul_converted].
-        rewrite Rows.flatten_partitions with (n:=n3) by (eauto using Rows.length_from_associational; omega).
-        autorewrite with distr_length push_eval natsimplify.
-        rewrite w_0; autorewrite with zsimplify.
-        reflexivity.
+        rewrite from_associational_partitions by auto. push_eval.
       Qed.
 
-      Lemma mul_converted_div n1 n2 m1 m2 n3 idxs p1 p2:
-        m1 <> 0%nat -> m2 <> 0%nat -> n3 = 2%nat ->
-        length p1 = n1 -> length p2 = n2 ->
-        0 <= Positional.eval w n1 p1  ->
-        0 <= Positional.eval w n2 p2  ->
-        0 <= (Positional.eval w n1 p1 * Positional.eval w n2 p2) < w n3 ->
-        nth_default 0 (mul_converted n1 n2 m1 m2 n3 idxs p1 p2) 1 = (Positional.eval w n1 p1 * Positional.eval w n2 p2) / (w 1).
+      Lemma from_associational_eq n idxs p  (_:n<>0%nat):
+        from_associational idxs n p = Rows.partition w n (Associational.eval p).
       Proof.
-        intros; subst n3; cbv [mul_converted].
-        rewrite Rows.flatten_partitions with (n:=2%nat) by (eauto using Rows.length_from_associational; omega).
-        autorewrite with distr_length push_eval.
-        rewrite Z.mod_small; omega.
+        intros. cbv [from_associational].
+        rewrite Rows.flatten_partitions' with (n:=n) by eauto using Rows.length_from_associational.
+        push_eval.
+      Qed.
+        
+      (* TODO: convert all _partitions proofs to this form? *)
+      Lemma mul_converted_eq n1 n2 m1 m2 n3 idxs p1 p2  (_:n3<>0%nat) (_:m1<>0%nat) (_:m2<>0%nat):
+        length p1 = n1 -> length p2 = n2 ->
+        mul_converted n1 n2 m1 m2 n3 idxs p1 p2 = Rows.partition w n3 (Positional.eval w n1 p1 * Positional.eval w n2 p2).
+      Proof.
+        intros; cbv [mul_converted].
+        rewrite from_associational_eq by auto. push_eval.
       Qed.
 
-      (* shortcut definition for convert-mul-convert for cases when we are halving the bitwidth before multiplying. *)
-      (* the most important feature here is the carries--we carry from all the odd indices after multiplying,
-         thus pre-aligning everything with the double-size bitwidth *)
-      Definition mul_converted_halve n n2 :=
-        mul_converted n n n2 n2 n2 (map (fun x => 2*x + 1)%nat (seq 0 n)).
+      Section aligned.
+        Context (log_w'_w : nat) (Hlog_w'_w : forall i, (w' i) ^ Z.of_nat log_w'_w = w i).
+        Context (n n' nout : nat) (Hn : n <> 0%nat) (Hn' : n' <> 0%nat) (Hnout : nout <> 0%nat).
+        
+        (* carry chain that aligns terms in the intermediate weight with the final weight *)
+        Definition aligned_carries := (map (fun i => ((log_w'_w * (i + 1)) - 1))%nat (seq 0 nout)).
+        
+        Definition from_associational_aligned := from_associational aligned_carries nout.
+        
+        (* assumes both inputs have the same length *)
+        Definition mul_aligned := mul_converted n n n' n' nout aligned_carries.
 
+        Lemma mul_aligned_eq p1 p2 :
+          length p1 = n -> length p2 = n ->
+          mul_aligned p1 p2 = Rows.partition w nout (Positional.eval w n p1 * Positional.eval w n p2).
+        Proof. cbv [mul_aligned aligned_carries]. auto using mul_converted_eq. Qed.
+
+        Lemma eval_mul_aligned p1 p2 :
+          length p1 = n -> length p2 = n ->
+          0 <= Positional.eval w n p1 * Positional.eval w n p2 < w nout ->
+          Positional.eval w nout (mul_aligned p1 p2) = Positional.eval w n p1 * Positional.eval w n p2.
+        Proof. cbv [mul_aligned aligned_carries]. auto using eval_mul_converted. Qed.
+      End aligned.
   End mul_converted.
 End MulConverted.
 
@@ -7655,14 +7823,11 @@ Module MontgomeryReduction.
     Let w_mul_1_gt1 : w_mul 1 > 1 := weight_1_gt_1 _ _ half_log2R_good.
     Context (nout : nat) (Hnout : nout = 2%nat).
 
-    (* simpler version of mul_converted with a carry chain that aligns
-      terms in the intermediate weight with the final weight *)
-    Definition mul_converted_aligned w w' (log_w'_w : nat) n m nout :=
-      MulConverted.mul_converted w w' n n m m nout (map (fun i => ((log_w'_w * (i + 1)) - 1))%nat (seq 0 nout)).
+    Definition widemul a b := MulConverted.mul_aligned w w_mul n 1%nat n nout [a] [b].
 
     Definition montred' (lo_hi : (Z * Z)) :=
-      dlet_nd y := nth_default 0 (mul_converted_aligned w w_mul n 1%nat n nout [fst lo_hi] [N']) 0  in
-      dlet_nd t1_t2 := mul_converted_aligned w w_mul n 1%nat n nout [y] [N] in
+      dlet_nd y := nth_default 0 (widemul (fst lo_hi) N') 0  in
+      dlet_nd t1_t2 := widemul y N in
       dlet_nd lo'_carry := Z.add_get_carry_full R (fst lo_hi) (nth_default 0 t1_t2 0) in
       dlet_nd hi'_carry := Z.add_with_get_carry_full R (snd lo'_carry) (snd lo_hi) (nth_default 0 t1_t2 1) in
       dlet_nd y' := Z.zselect (snd hi'_carry) 0 N in
@@ -7676,9 +7841,10 @@ Module MontgomeryReduction.
       rewrite Z.pow_mul_r, R_two_pow by omega; reflexivity.
     Qed.
 
+    Local Ltac change_weight := rewrite !Hw, ?Z.pow_0_r, ?Z.pow_1_r, ?Z.pow_2_r in *.
     Local Ltac solve_range :=
       repeat match goal with
-             | _ => rewrite Hw, ?Z.pow_0_r, ?Z.pow_1_r, ?Z.pow_2_r
+             | _ => progress change_weight
              | |- context [?a mod ?b] => unique pose proof (Z.mod_pos_bound a b ltac:(omega))
              | |- 0 <= _ => progress Z.zero_bounds
              | |- 0 <= _ * _ < _ * _ =>
@@ -7688,9 +7854,14 @@ Module MontgomeryReduction.
              | _ => nia
              end.
 
-    Hint Rewrite
-         MulConverted.mul_converted_mod MulConverted.mul_converted_div using (solve [auto; autorewrite with mul_conv; solve_range])
-      : mul_conv.
+    Lemma widemul_correct x y :
+      0 <= x * y < w 2 -> widemul x y = [(x * y) mod R; (x * y) / R].
+    Proof.
+      intros; cbv [widemul]. rewrite MulConverted.mul_aligned_eq by (auto; distr_length).
+      subst nout. cbn. change_weight.
+      autorewrite with zsimplify.
+      Z.rewrite_mod_small. reflexivity.
+    Qed.
 
     Lemma montred'_eq lo_hi T (HT_range: 0 <= T < R * N)
           (Hlo: fst lo_hi = T mod R) (Hhi: snd lo_hi = T / R):
@@ -7698,11 +7869,11 @@ Module MontgomeryReduction.
     Proof.
       rewrite <-reduce_via_partial_alt_eq by nia.
       cbv [montred' partial_reduce_alt reduce_via_partial_alt prereduce Let_In].
-      rewrite Hlo, Hhi. subst nout.
+      rewrite Hlo, Hhi.
       assert (0 <= T mod R * N' < w 2) by (solve_range).
-      cbv [mul_converted_aligned]. cbn [seq map].
-      autorewrite with mul_conv.
-      rewrite Hw, ?Z.pow_1_r.
+
+      rewrite !widemul_correct by (rewrite ?widemul_correct; autorewrite with push_nth_default; solve_range).
+      autorewrite with push_nth_default.
       autorewrite with to_div_mod. rewrite ?Z.zselect_correct, ?Z.add_modulo_correct.
 
       (* pull out value before last modular reduction *)
@@ -7713,8 +7884,7 @@ Module MontgomeryReduction.
         |- context [if R * R <=? ?x then _ else _] =>
         match goal with |- context [if dec (?xHigh / R = 0) then _ else _] =>
                         assert (x / R = xHigh) as cond_equiv end end.
-      { apply Z.mul_cancel_r with (p:=R); [omega|]. cbn.
-        rewrite w_0. autorewrite with zsimplify_fast.
+      { apply Z.mul_cancel_r with (p:=R); [omega|].
         autorewrite with push_Zmul zdiv_to_mod push_Zmod; ring. }
       rewrite <-cond_equiv. rewrite ?Z.mod_pull_div, ?Z.div_div by omega.
       assert (0 < R * R)%Z by Z.zero_bounds.
@@ -7762,7 +7932,7 @@ Module MontgomeryReduction.
     Let bound := Some r[0 ~> (2^machine_wordsize - 1)%Z]%zrange.
 
     Definition relax_zrange_of_machine_wordsize
-      := relax_zrange_gen [1; machine_wordsize / 2; machine_wordsize; 2 * machine_wordsize; 4 * machine_wordsize]%Z.
+      := relax_zrange_gen [1; machine_wordsize / 2; machine_wordsize; 2 * machine_wordsize]%Z.
     Local Arguments relax_zrange_of_machine_wordsize / .
 
     Let relax_zrange := relax_zrange_of_machine_wordsize.
@@ -7855,7 +8025,7 @@ montred256 = fun var : type -> Type => λ x : var (type.type_primitive type.Z * 
              expr_let x29 := SELC (x28₂, 0, 115792089210356248762697446949407573530086143415290314195533631308867097853951) in
              expr_let x30 := Z.cast uint256 @@ (fst @@ SUB_256 (x28₁, x29)) in
              ADDM (x30, 0, 115792089210356248762697446949407573530086143415290314195533631308867097853951)
-     : Expr (type.type_primitive type.Z * type.type_primitive type.Z -> type.type_primitive type.Z)
+     : Expr (type.uncurry (type.type_primitive type.Z * type.type_primitive type.Z -> type.type_primitive type.Z))
    *)
 End Montgomery256.
 
@@ -7881,10 +8051,10 @@ Module Montgomery256PrintingNotations.
     (AppIdent
        (primitive 79228162514264337593543950335)
        TT) (only printing, at level 9) : expr_scope.
-  Notation "'RegMod' '<<' '128'" :=
+  Notation "'RegMod' '>>' '128'" :=
     (AppIdent
        (primitive 340282366841710300967557013911933812736)
-       TT) (only printing, at level 9, format "'RegMod'  '<<'  '128'") : expr_scope.
+       TT) (only printing, at level 9, format "'RegMod'  '>>'  '128'") : expr_scope.
   Notation "'Lower128{RegPinv}'" :=
     (AppIdent
        (primitive 79228162514264337593543950337)
@@ -7981,7 +8151,7 @@ c.Lower128($x12, $x10_lo);
 c.Mul128x128($x13, Lower128{RegMod}, $x11);
 c.ShiftR($x14, $x13, 128);
 c.Lower128($x15, $x13);
-c.Mul128x128($x16, RegMod << 128, $x12);
+c.Mul128x128($x16, RegMod >> 128, $x12);
 c.ShiftR($x17, $x16, 128);
 c.Lower128($x18, $x16);
 c.ShiftL($x19, $x18, 128);
@@ -7990,7 +8160,7 @@ c.Add256($x21, $x19, $x20);
 c.Addc($x22, $x14, $x17);
 c.ShiftL($x23, $x15, 128);
 c.Add256($x24, $x23, $x21_lo);
-c.Mul128x128($x25, RegMod << 128, $x11);
+c.Mul128x128($x25, RegMod >> 128, $x11);
 c.Addc($x26, $x25, $x22_lo);
 c.Add256($x27, $x_lo, $x24_lo);
 c.Addc($x28, $x_hi, $x26_lo);
